More inlining.
Could do without the intermediate games given a generic way of turning
equiv goals on statements into equiv goals on oracle calls
(syntactic equality).

examples/PSS.ec
@@ -181,6 +181,23 @@ module type CMA_2RO(G:Gt.ARO,H:Ht.ARO,S:AdvOracles) = {
 
 section.
 declare module G:Gt.Oracle {EF_CMA.WrapEF,Gt.WRO_Set.ARO,Ht.WRO_Set.ARO}.
+
+module Correct_G(G:Gt.Oracle) = {
+  fun call2(x:htag): gtag * gtag = {
+    var g, g':gtag;
+    g = G.o(x);
+    g' = G.o(x);
+    return (g,g');
+  }
+
+  fun call1(x:htag): gtag = {
+    var g:gtag;
+    g = G.o(x);
+    return g;
+  } 
+}.
+axiom correct_G: equiv [Correct_G(G).call2 ~ Correct_G(G).call1: ={x, glob G} ==> ={glob G} /\ res{1} = (res,res){2}].
+
 declare module H:Ht.Oracle {EF_CMA.WrapEF,Ht.WRO_Set.ARO,Gt.WRO_Set.ARO(G)}.
 
 declare module Adv:CMA_2RO {Gt.WRO_Set.ARO(G),Ht.WRO_Set.ARO(H),EF_CMA.WrapEF(PSS(G,H))}.
@@ -188,7 +205,191 @@ axiom AdvL (G<:Gt.Oracle) (H<:Ht.Oracle):
   islossless G.o => islossless H.o =>
   islossless Adv(Gt.WRO_Set.ARO(G),Ht.WRO_Set.ARO(H),EF_CMA.WrapEF(PSS(G,H))).forge.
 
-local module G0(G:Gt.Oracle,H:Ht.Oracle): PKSi.EF_CMA.Oracles = {
+(* Folding in the two calls to G *)
+module PSS'(G:Gt.Oracle,H:Ht.Oracle): Scheme = {
+  module G2 = Correct_G(G)
+  module G' = Gt.WRO_Set.ARO(G)
+  module H' = Ht.WRO_Set.ARO(H)
+
+  fun init(): unit = {
+    H'.init();
+    G'.init();
+  }
+
+  (* Keygen: make it a wrapped pop *)
+  fun keygen():(pkey * skey) = {
+    var (pk, sk):(pkey * skey);
+    (pk,sk) = $keypairs;
+    return (pk,sk);
+  }
+
+  (* Sign *)
+  fun sign(sk:skey, m:message):signature = {
+    var r:salt;
+    var g,g':gtag;
+    var rMask:salt;
+    var maskedR:salt;
+    var w:htag;
+    var gamma:g2tag;
+    var y:signature;
+
+    r = $sample_salt;
+    w  = H.o(m || (to_bits r));
+    (g,g') = G2.call2(w);
+    rMask = Salt.from_bits (sub (to_bits g) 0 k0);
+    maskedR = rMask ^ r;
+    gamma  = G2Tag.from_bits (sub (to_bits g') k0 kg2);
+    y = Signature.from_bits (zeros 1 || (to_bits w) || (to_bits maskedR) || (to_bits gamma));
+    return (finv sk y); (* For fault injection, we will later refine this; we should make it a function so it can be reasoned about separately *)
+  }
+
+  (* Verify *)
+  fun verify(pk:pkey, m:message, s:signature):bool = {
+    var y:signature;
+    var g, g':gtag;
+    var w:htag;
+    var w':htag;
+    var maskedR:salt;
+    var gamma:g2tag;
+    var gamma':g2tag;
+    var rMask:salt;
+    var r:salt;
+    var b:bool;
+
+    y = (f pk s);
+    b = (sub (to_bits y) 0 1 <> zeros 1);
+    w = HTag.from_bits (sub (to_bits y) 1 k1);
+    maskedR = Salt.from_bits (sub (to_bits y) (k1 + 1) k0);
+    gamma = G2Tag.from_bits (sub (to_bits y) (k1 + k0 + 1) kg2);
+    (g,g') = G2.call2(w);
+    rMask  = Salt.from_bits (sub (to_bits g) 0 k0);
+    r = rMask ^ maskedR;
+    w'  = H.o(m || to_bits r);
+    gamma'  = G2Tag.from_bits (sub (to_bits g') k0 kg2);
+    return (w = w' /\ gamma = gamma' /\ !b);
+  }
+}.
+
+local equiv PSS_PSS':
+  PKSi.EF_CMA.EF_CMA(EF_CMA.WrapEF(PSS(G,H)),Adv(Gt.WRO_Set.ARO(G),Ht.WRO_Set.ARO(H))).main ~
+  PKSi.EF_CMA.EF_CMA(EF_CMA.WrapEF(PSS'(G,H)),Adv(Gt.WRO_Set.ARO(G),Ht.WRO_Set.ARO(H))).main:
+  ={glob Adv} ==> ={res}.
+proof.
+fun.
+call (_: ={EF_CMA.WrapEF.qs, m} ==> ={res});
+  first by fun; wp.
+call (_: ={glob H, glob G, EF_CMA.WrapEF.pk, m, s} ==> ={res});
+  first by fun; call (_: ={glob H, glob G, EF_CMA.WrapEF.pk, pk, m, s} ==> ={res})=> //;
+             fun; inline PSS(G,H).g1 PSS(G,H).g2 PSS'(G,H).G2.call2;
+                  swap{1} 11 -4; swap{1} 12 -3; eqobs_in; wp; eqobs_in.
+call (_: ={glob H, glob G, glob EF_CMA.WrapEF, glob Gt.WRO_Set.ARO, glob Ht.WRO_Set.ARO}).
+  fun; call (_: ={glob H, glob G, EF_CMA.WrapEF.sk, sk, m} ==> ={glob H, glob G, EF_CMA.WrapEF.sk, res});
+    last by wp.
+    fun; inline PSS(G,H).g1 PSS(G,H).g2 PSS'(G,H).G2.call2;
+         swap{1} 7 -3; swap{1} 8 -2; eqobs_in; wp; eqobs_in.
+  by fun; eqobs_in.
+  by fun; eqobs_in.
+call (_: true ==> ={glob Ht.WRO_Set.ARO(H), glob Gt.WRO_Set.ARO(G), glob EF_CMA.WrapEF, res})=> //.
+  by fun; eqobs_in.
+qed.
+
+module PSS''(G:Gt.Oracle,H:Ht.Oracle): Scheme = {
+  module G2 = Correct_G(G)
+  module G' = Gt.WRO_Set.ARO(G)
+  module H' = Ht.WRO_Set.ARO(H)
+
+  fun init(): unit = {
+    H'.init();
+    G'.init();
+  }
+
+  (* Keygen: make it a wrapped pop *)
+  fun keygen():(pkey * skey) = {
+    var (pk, sk):(pkey * skey);
+    (pk,sk) = $keypairs;
+    return (pk,sk);
+  }
+
+  (* Sign *)
+  fun sign(sk:skey, m:message):signature = {
+    var r:salt;
+    var g:gtag;
+    var rMask:salt;
+    var maskedR:salt;
+    var w:htag;
+    var gamma:g2tag;
+    var y:signature;
+
+    r = $sample_salt;
+    w  = H.o(m || (to_bits r));
+    g = G2.call1(w);
+    rMask = Salt.from_bits (sub (to_bits g) 0 k0);
+    maskedR = rMask ^ r;
+    gamma  = G2Tag.from_bits (sub (to_bits g) k0 kg2);
+    y = Signature.from_bits (zeros 1 || (to_bits w) || (to_bits maskedR) || (to_bits gamma));
+    return (finv sk y); (* For fault injection, we will later refine this; we should make it a function so it can be reasoned about separately *)
+  }
+
+  (* Verify *)
+  fun verify(pk:pkey, m:message, s:signature):bool = {
+    var y:signature;
+    var g:gtag;
+    var w:htag;
+    var w':htag;
+    var maskedR:salt;
+    var gamma:g2tag;
+    var gamma':g2tag;
+    var rMask:salt;
+    var r:salt;
+    var b:bool;
+
+    y = (f pk s);
+    b = (sub (to_bits y) 0 1 <> zeros 1);
+    w = HTag.from_bits (sub (to_bits y) 1 k1);
+    maskedR = Salt.from_bits (sub (to_bits y) (k1 + 1) k0);
+    gamma = G2Tag.from_bits (sub (to_bits y) (k1 + k0 + 1) kg2);
+    g = G2.call1(w);
+    rMask  = Salt.from_bits (sub (to_bits g) 0 k0);
+    r = rMask ^ maskedR;
+    w'  = H.o(m || to_bits r);
+    gamma'  = G2Tag.from_bits (sub (to_bits g) k0 kg2);
+    return (w = w' /\ gamma = gamma' /\ !b);
+  }
+}.
+
+local equiv PSS'_PSS'':
+  PKSi.EF_CMA.EF_CMA(EF_CMA.WrapEF(PSS'(G,H)),Adv(Gt.WRO_Set.ARO(G),Ht.WRO_Set.ARO(H))).main ~
+  PKSi.EF_CMA.EF_CMA(EF_CMA.WrapEF(PSS''(G,H)),Adv(Gt.WRO_Set.ARO(G),Ht.WRO_Set.ARO(H))).main:
+  ={glob Adv} ==> ={res}.
+proof.
+fun.
+call (_: ={EF_CMA.WrapEF.qs, m} ==> ={res});
+  first by fun; wp.
+call (_: ={glob H, glob G, EF_CMA.WrapEF.pk, m, s} ==> ={res});
+  first by fun; call (_: ={glob H, glob G, EF_CMA.WrapEF.pk, pk, m, s} ==> ={res})=> //;
+             fun; eqobs_in; call correct_G; wp.
+call (_: ={glob H, glob G, glob EF_CMA.WrapEF, glob Gt.WRO_Set.ARO, glob Ht.WRO_Set.ARO}).
+  fun; call (_: ={glob H, glob G, EF_CMA.WrapEF.sk, sk, m} ==> ={glob H, glob G, EF_CMA.WrapEF.sk, res});
+    last by wp.
+    fun; eqobs_in; call correct_G; wp;
+    call (_: ={glob H, x} ==> ={glob H, res});
+      first by fun (true).
+    by rnd.
+  by fun; eqobs_in.
+  by fun; eqobs_in.
+call (_: true ==> ={glob Ht.WRO_Set.ARO(H), glob Gt.WRO_Set.ARO(G), glob EF_CMA.WrapEF, res})=> //;
+  by fun; eqobs_in.
+qed.
+
+(** EF-CMA security of PSS *)
+(* A CMA adversary with access to two random oracles *)
+module type PartialOracles(G:Gt.Oracle,H:Ht.Oracle) = {
+  fun init(): pkey
+  fun sign(m:message): signature
+  fun fresh(m:message): bool
+}.
+
+local module G0o(G:Gt.Oracle,H:Ht.Oracle): PartialOracles(G H) = {
   module G' = Gt.WRO_Set.ARO(G)
   module H' = Ht.WRO_Set.ARO(H)
 
@@ -205,20 +406,9 @@ local module G0(G:Gt.Oracle,H:Ht.Oracle): PKSi.EF_CMA.Oracles = {
     return pk;
   }
 
-  fun g1(x:htag): salt = {
-    var r:gtag;
-    r = G.o(x);
-    return Salt.from_bits (sub (to_bits r) 0 k0);
-  }
-
-  fun g2(x:htag): g2tag = {
-    var r:gtag;
-    r = G.o(x);
-    return G2Tag.from_bits (sub (to_bits r) k0 kg2);
-  }
-
   fun sign(m:message): signature = {
     var r:salt;
+    var g:gtag;
     var rMask:salt;
     var maskedR:salt;
     var w:htag;
@@ -228,86 +418,105 @@ local module G0(G:Gt.Oracle,H:Ht.Oracle): PKSi.EF_CMA.Oracles = {
     qs = add m qs;
     r = $sample_salt;
     w  = H.o(m || (to_bits r));
-    rMask  = g1(w);
+    g = G.o(w);
+    rMask  = Salt.from_bits (sub (to_bits g) 0 k0);
     maskedR = rMask ^ r;
-    gamma  = g2(w);
+    gamma  = G2Tag.from_bits (sub (to_bits g) k0 kg2);
     y = Signature.from_bits (zeros 1 || (to_bits w) || (to_bits maskedR) || (to_bits gamma));
     return finv sk y;
-  }
-
-  fun verify(m:message,s:signature): bool = {
-    var y:signature;
-    var w:htag;
-    var w':htag;
-    var maskedR:salt;
-    var gamma:g2tag;
-    var gamma':g2tag;
-    var rMask:salt;
-    var r:salt;
-    var b:bool;
-
-    y = (f pk s);
-    b = (sub (to_bits y) 0 1 <> zeros 1);
-    w = HTag.from_bits (sub (to_bits y) 1 k1);
-    maskedR = Salt.from_bits (sub (to_bits y) (k1 + 1) k0);
-    gamma = G2Tag.from_bits (sub (to_bits y) (k1 + k0 + 1) kg2);
-    rMask  = g1(w);
-    r = rMask ^ maskedR;
-    w'  = H.o(m || to_bits r);
-    gamma'  = g2(w);
-    return (w = w' /\ gamma = gamma' /\ !b);
-  }
+  } 
 
   fun fresh(m:message): bool = {
     return !mem m qs;
   }
 }.
 
+local module G0(G:Gt.Oracle,H:Ht.Oracle,O:PartialOracles,A:CMA_2RO) = {
+  module O = O(G,H)
+  module A = A(Gt.WRO_Set.ARO(G),Ht.WRO_Set.ARO(H),O)
+
+  fun main(): bool = {
+    var pk:pkey;
+    var m:message;
+    var s:signature;
+    var y:signature;
+    var w:htag;
+    var w':htag;
+    var g:gtag;
+    var maskedR:salt;
+    var gamma:g2tag;
+    var gamma':g2tag;
+    var rMask:salt;
+    var r:salt;
+    var forged, fresh:bool;
+
+    pk = O.init();
+    (m,s) = A.forge(pk);
+
+    y = (f pk s);
+    forged = (sub (to_bits y) 0 1 <> zeros 1);
+    w = HTag.from_bits (sub (to_bits y) 1 k1);
+    maskedR = Salt.from_bits (sub (to_bits y) (k1 + 1) k0);
+    gamma = G2Tag.from_bits (sub (to_bits y) (k1 + k0 + 1) kg2);
+    g = G.o(w);
+    rMask  = Salt.from_bits (sub (to_bits g) 0 k0);
+    r = rMask ^ maskedR;
+    w'  = H.o(m || to_bits r);
+    gamma'  = G2Tag.from_bits (sub (to_bits g) k0 kg2);
+    forged =  w = w' /\ gamma = gamma' /\ !forged;
+
+    fresh = O.fresh(m);
+    return forged /\ fresh;
+  }
+}.
+
 local module PSSi = PSS(G,H).
 local module PSSo = EF_CMA.WrapEF(PSSi).
-local module G0o  = G0(G,H).
 
-local lemma PSS_G0_fresh:
-  equiv [PSSo.fresh ~ G0o.fresh: ={m} /\ PSSo.qs{1} = G0o.qs{2} ==> ={res}]
+local lemma PSS''_G0_fresh:
+  equiv [EF_CMA.WrapEF(PSS''(G,H)).fresh ~ G0o(G,H).fresh: ={m} /\ PSSo.qs{1} = G0o.qs{2} ==> ={res}]
 by by fun.
 
-local lemma PSS_G0_verify:
-  equiv [PSSo.verify ~ G0o.verify: ={m,s,glob G,glob H} /\ PSSo.pk{1} = G0o.pk{2} ==> ={res}].
+(*local lemma PSS_G0_verify:
+  equiv [PSSo.verify ~ G0o'.verify: ={m,s,glob G,glob H} /\ PSSo.pk{1} = G0o'.pk{2} ==> ={res}].
 proof.
 fun; inline PSS(G,H).verify;
 seq 12 9: (={w,w',gamma,gamma'} /\ b0{1} = b{2}); last by wp.
 eqobs_in.
-qed.
+qed.*)
 
-local lemma PSS_G0_sign:
-  equiv [PSSo.sign ~ G0o.sign:
-    ={m,glob G,glob H} /\ PSSo.sk{1} = G0o.sk{2} /\ PSSo.qs{1} = G0o.qs{2} ==>
-    ={glob G,glob H,res} /\ PSSo.sk{1} = G0o.sk{2} /\ PSSo.qs{1} = G0o.qs{2}].
+local lemma PSS''_G0_sign:
+  equiv [EF_CMA.WrapEF(PSS''(G,H)).sign ~ G0o(G,H).sign:
+    ={m,glob G, glob H} /\ EF_CMA.WrapEF.qs{1} = G0o.qs{2} /\ EF_CMA.WrapEF.sk{1} = G0o.sk{2} ==>
+    ={glob G,glob H, res} /\ EF_CMA.WrapEF.qs{1} = G0o.qs{2} /\ EF_CMA.WrapEF.sk{1} = G0o.sk{2}].
 proof.
-fun; inline PSS(G,H).sign.
-seq 9 7: (={glob G, glob H, y} /\
-          PSSo.sk{1} = G0o.sk{2} /\
-          PSSo.qs{1} = G0o.qs{2} /\
-          sk{1} = G0o.sk{2}).
+fun; inline PSS''(G,H).sign PSS''(G,H).G2.call1.
+seq 12 8: (={glob G, glob H, y} /\
+           EF_CMA.WrapEF.qs{1} = G0o.qs{2} /\
+           EF_CMA.WrapEF.sk{1} = G0o.sk{2} /\
+           sk{1} = G0o.sk{2}).
   by eqobs_in.
   by wp.
 qed.
 
-local module PSS_G' = PSS(G,H).G'.
-local module PSS_H' = PSS(G,H).H'.
-local module G0_G' = G0(G,H).G'.
-local module G0_H' = G0(G,H).H'.
+local module PSS_G' = PSS''(G,H).G'.
+local module PSS_H' = PSS''(G,H).H'.
+local module G0_G' = G0o(G,H).G'.
+local module G0_H' = G0o(G,H).H'.
 
-local equiv PSS_G0_init: PSSo.init ~ G0o.init:
+local module PSSo'' = EF_CMA.WrapEF(PSS''(G,H)).
+
+local equiv PSS''_G0_init: PSSo''.init ~ G0o(G,H).init:
   true ==>
   ={res} /\
-  PSSo.qs{1} = G0o.qs{2} /\
+  PSSo''.qs{1} = G0o.qs{2} /\
   (glob PSS_G'){1} = (glob G0_G'){2} /\
   (glob PSS_H'){1} = (glob G0_H'){2} /\
-  PSSo.pk{1} = G0o.pk{2} /\
-  PSSo.sk{1} = G0o.sk{2}.
+  PSSo''.pk{1} = G0o.pk{2} /\
+  PSSo''.sk{1} = G0o.sk{2} /\
+  G0o.pk{2} = res{2}.
 proof.
-fun; inline PSS(G,H).keygen PSS(G,H).init.
+fun. inline PSS''(G,H).init PSS''(G,H).keygen PSS(G,H).init.
 wp; rnd; wp.
 seq 2 2: ((glob PSS_G'){1} = (glob G0_G'){2} /\
           (glob PSS_H'){1} = (glob G0_H'){2})=> //.
@@ -317,31 +526,35 @@ call (_: true ==> (glob PSS_H'){1} = (glob G0_H'){2})=> //;
   first by fun; wp; call (_: true ==> ={glob H})=> //; fun (true)=> //.
 qed.
 
-local lemma PSS_G0:
-  equiv [PKSi.EF_CMA.EF_CMA(PSSo,Adv(Gt.WRO_Set.ARO(G),Ht.WRO_Set.ARO(H))).main ~
-         PKSi.EF_CMA.EF_CMA(G0o,Adv(Gt.WRO_Set.ARO(G),Ht.WRO_Set.ARO(H))).main:
+local lemma PSS''_G0:
+  equiv [PKSi.EF_CMA.EF_CMA(PSSo'',Adv(Gt.WRO_Set.ARO(G),Ht.WRO_Set.ARO(H))).main ~
+         G0(G,H,G0o,Adv).main:
            ={glob Adv} ==> ={res}].
 proof.
 fun;
-call PSS_G0_fresh.
-call PSS_G0_verify.
-call (_: (glob PSS_G'){1} = (glob G0_G'){2} /\
-         (glob PSS_H'){1} = (glob G0_H'){2} /\
-         ={glob Adv, pk} /\
-         PSSo.sk{1} = G0o.sk{2} /\
-         PSSo.qs{1} = G0o.qs{2} ==>
-         (glob PSS_G'){1} = (glob G0_G'){2} /\
-         (glob PSS_H'){1} = (glob G0_H'){2} /\
-         PSSo.qs{1} = G0o.qs{2} /\
-         ={res}).
-  fun ((glob PSS_G'){1} = (glob G0_G'){2} /\
-       (glob PSS_H'){1} = (glob G0_H'){2} /\
-       PSSo.sk{1} = G0o.sk{2} /\
-       PSSo.qs{1} = G0o.qs{2})=> //.
-    by conseq* PSS_G0_sign.
+call PSS''_G0_fresh.
+seq 2 2: (={glob Gt.WRO_Set.ARO(G), glob Ht.WRO_Set.ARO(H), m, s} /\
+          EF_CMA.WrapEF.qs{1} = G0o.qs{2} /\
+          EF_CMA.WrapEF.pk{1} = G0o.pk{2} /\
+          G0o.pk{2} = pk{2}).
+  call (_: ={glob Gt.WRO_Set.ARO(G), glob Ht.WRO_Set.ARO(H)} /\
+           EF_CMA.WrapEF.qs{1} = G0o.qs{2} /\
+           EF_CMA.WrapEF.pk{1} = G0o.pk{2} /\
+           EF_CMA.WrapEF.sk{1} = G0o.sk{2}).
+    by conseq* PSS''_G0_sign.
     by fun; eqobs_in.
     by fun; eqobs_in.
-by call PSS_G0_init.
+  by call PSS''_G0_init.
+inline EF_CMA.WrapEF(PSS''(G,H)).verify PSS''(G,H).verify PSS''(G,H).G2.call1.
+conseq * (_: ={glob H, glob G, m, s} /\ EF_CMA.WrapEF.pk{1} = G0o.pk{2} /\ G0o.pk{2} = pk{2} ==>
+             ={glob H, glob G, forged} /\ EF_CMA.WrapEF.pk{1} = G0o.pk{2})=> //.
+wp.
+call (_: ={glob H, x} ==> ={glob H, res});
+  first by fun (true).
+wp.
+call (_: ={glob G, x} ==> ={glob G, res});
+  first by fun (true).
+by wp; skip.
 qed.
 
 (* PROOF GOES HERE *)
